\def\arraystretch{3}
{\normalsize
  \begin{center}
    \begin{tabular}{| >{\centering}m{5cm}| >{\centering}m{5cm}| >{\centering}m{5cm}|}
      \hline
      $\sum_{k = 0}^n k = \frac{n(n + 1)}{2}$
       &
      $\sum_{k = 0}^n k^2 = \frac{n(n + 1)(2n + 1)}{6}$
       &
      $\sum_{k = 0}^n k^3 = \frac{n^2(n + 1)^2}{4}$
      \tabularnewline \hline
      $\sum_{k = 0}^n a^k = \frac{1 - a^{n + 1}}{1 - a}$
       &
      $\sum_{k = 0}^n ka^k = \frac{a[1 - (n + 1)a^n + na^{n + 1}]}{(1 - a)^2}$
       &
      $ a + b = a \oplus b + 2(a \& b)$
      \tabularnewline \hline
      $\sum_{k = 0}^\infty a^k = \frac{1}{1 - a}, |a| < 1$
       &
      $\sum_{k = 0}^\infty ka^k = \frac{a}{(1 - a)^2}, |a| < 1$
       &
      $\sum_{k = 0}^\infty k^2a^k = \frac{a^2 + a}{(1 - a)^3}, |a| < 1$
      \tabularnewline \hline
      $\sum_{k = 0}^\infty \frac{1}{a^k} = \frac{a}{a - 1}, |a| > 1$
       &
      $\sum_{k = 0}^n \binom{n}{k} a^k b^{n-k} = (a+b)^n $
       &
      $\sum_{k = 0}^\infty \frac{k^2}{a^k} = \frac{a^2 + a}{(a - 1)^3}, |a| > 1$
      \tabularnewline \hline
      $\sum_{k = 0}^\infty \frac{a^k}{k!} = e^a$
       &
      $\sum_{k = 0}^n \binom{n}{k} = 2^n$
       &
      $\sum_{k = 0}^n \binom{k}{m} = \binom{n + 1}{m + 1}$
      \tabularnewline \hline
    \end{tabular}
  \end{center}
}
